Phi_System/IDE_CP_Applications1.thy
@@ -630,54 +630,67 @@ lemma [\<phi>reason 1200]:
 
 subsection \<open>Case Analysis\<close>
 
-consts \<A>_action_case :: \<open>action\<close>
-       \<A>_action_case_on :: \<open>action\<close>
+consts \<A>case :: \<open>'a \<Rightarrow> action\<close>
 
-lemma cases_\<phi>app: \<open>PROP Call_Action (\<A>_view_shift_or_imp \<A>_action_case)\<close> ..
-lemma cases_on_\<phi>app: \<open>PROP Call_Action (\<A>_view_shift_or_imp \<A>_action_case_on)\<close> ..
+
+lemma "_cases_app_rule_":
+  \<open>Call_Action (\<A>_view_shift_or_imp (\<A>case target))\<close>
+  for target :: 'a ..
+
+thm list.induct
 
 declare [[ \<phi>reason_default_pattern
-      \<open>?X \<t>\<r>\<a>\<n>\<s>\<f>\<o>\<r>\<m>\<s> _ \<w>\<i>\<t>\<h> _ @action \<A>_action_case\<close> \<Rightarrow>
-      \<open>?X \<t>\<r>\<a>\<n>\<s>\<f>\<o>\<r>\<m>\<s> _ \<w>\<i>\<t>\<h> _ @action \<A>_action_case\<close>    (100)
-  and \<open>?X \<s>\<h>\<i>\<f>\<t>\<s>  _ \<w>\<i>\<t>\<h> _ @action \<A>_action_case\<close> \<Rightarrow>
-      \<open>?X \<s>\<h>\<i>\<f>\<t>\<s>  _ \<w>\<i>\<t>\<h> _ @action \<A>_action_case\<close>    (100)
-  and \<open>?X \<t>\<r>\<a>\<n>\<s>\<f>\<o>\<r>\<m>\<s> _ \<w>\<i>\<t>\<h> _ @action \<A>_action_case_on\<close> \<Rightarrow>
-      \<open>?X \<t>\<r>\<a>\<n>\<s>\<f>\<o>\<r>\<m>\<s> _ \<w>\<i>\<t>\<h> _ @action \<A>_action_case_on\<close>    (100)
-  and \<open>?X \<s>\<h>\<i>\<f>\<t>\<s>  _ \<w>\<i>\<t>\<h> _ @action \<A>_action_case_on\<close> \<Rightarrow>
-      \<open>?X \<s>\<h>\<i>\<f>\<t>\<s>  _ \<w>\<i>\<t>\<h> _ @action \<A>_action_case_on\<close>    (100)
+      \<open>?X \<t>\<r>\<a>\<n>\<s>\<f>\<o>\<r>\<m>\<s> _ \<w>\<i>\<t>\<h> _ @action \<A>case ?target\<close> \<Rightarrow>
+      \<open>?X \<t>\<r>\<a>\<n>\<s>\<f>\<o>\<r>\<m>\<s> _ \<w>\<i>\<t>\<h> _ @action \<A>case ?target\<close>    (100)
+  and \<open>?X \<s>\<h>\<i>\<f>\<t>\<s>  _ \<w>\<i>\<t>\<h> _ @action \<A>case ?target\<close> \<Rightarrow>
+      \<open>?X \<s>\<h>\<i>\<f>\<t>\<s>  _ \<w>\<i>\<t>\<h> _ @action \<A>case ?target\<close>    (100)
 ]]
 
-lemma [\<phi>reason 1000]:
+ML_file \<open>library/tools/induct_analysis.ML\<close>
+
+\<phi>processor case_analysis 5000 (\<open>_\<close>) \<open> IDECP_Induct_Analysis.case_analysis_processor \<close>
+
+
+lemma [\<phi>reason 1000 for \<open>_ + _ \<s>\<h>\<i>\<f>\<t>\<s> _ \<w>\<i>\<t>\<h> _ @action \<A>case (_ + _)\<close>
+                        \<open>_ + _ \<s>\<h>\<i>\<f>\<t>\<s> _ \<w>\<i>\<t>\<h> _ @action \<A>case ?var\<close>]:
   \<open> \<^bold>a\<^bold>r\<^bold>g\<^bold>u\<^bold>m\<^bold>e\<^bold>n\<^bold>t A \<s>\<h>\<i>\<f>\<t>\<s> Y \<w>\<i>\<t>\<h> PA
 \<Longrightarrow> \<^bold>a\<^bold>r\<^bold>g\<^bold>u\<^bold>m\<^bold>e\<^bold>n\<^bold>t B \<s>\<h>\<i>\<f>\<t>\<s> Y \<w>\<i>\<t>\<h> PB
-\<Longrightarrow> B + A \<s>\<h>\<i>\<f>\<t>\<s> Y \<w>\<i>\<t>\<h> PB \<or> PA @action \<A>_action_case\<close>
+\<Longrightarrow> B + A \<s>\<h>\<i>\<f>\<t>\<s> Y \<w>\<i>\<t>\<h> PB \<or> PA @action \<A>case (B + A)\<close>
   unfolding Argument_def Action_Tag_def using \<phi>CASE_VS .
 
-lemma [\<phi>reason 1000]:
+lemma [\<phi>reason 1000 for \<open>_ + _ \<t>\<r>\<a>\<n>\<s>\<f>\<o>\<r>\<m>\<s> _ \<w>\<i>\<t>\<h> _ @action \<A>case (_ + _)\<close>
+                        \<open>_ + _ \<t>\<r>\<a>\<n>\<s>\<f>\<o>\<r>\<m>\<s> _ \<w>\<i>\<t>\<h> _ @action \<A>case ?var\<close>]:
   \<open> \<^bold>a\<^bold>r\<^bold>g\<^bold>u\<^bold>m\<^bold>e\<^bold>n\<^bold>t A \<t>\<r>\<a>\<n>\<s>\<f>\<o>\<r>\<m>\<s> Y \<w>\<i>\<t>\<h> PA
 \<Longrightarrow> \<^bold>a\<^bold>r\<^bold>g\<^bold>u\<^bold>m\<^bold>e\<^bold>n\<^bold>t B \<t>\<r>\<a>\<n>\<s>\<f>\<o>\<r>\<m>\<s> Y \<w>\<i>\<t>\<h> PB
-\<Longrightarrow> B + A \<t>\<r>\<a>\<n>\<s>\<f>\<o>\<r>\<m>\<s> Y \<w>\<i>\<t>\<h> PB \<or> PA @action \<A>_action_case\<close>
+\<Longrightarrow> B + A \<t>\<r>\<a>\<n>\<s>\<f>\<o>\<r>\<m>\<s> Y \<w>\<i>\<t>\<h> PB \<or> PA @action \<A>case (B + A)\<close>
   unfolding Argument_def Action_Tag_def using \<phi>CASE_IMP .
 
-lemma [\<phi>reason 1000]:
+lemma [\<phi>reason 1000 for \<open>If _ _ _ \<s>\<h>\<i>\<f>\<t>\<s> _ \<w>\<i>\<t>\<h> _ @action \<A>case (If _ _ _)\<close>
+                        \<open>If _ _ _ \<s>\<h>\<i>\<f>\<t>\<s> _ \<w>\<i>\<t>\<h> _ @action \<A>case ?var\<close>]:
   \<open> (\<p>\<r>\<e>\<m>\<i>\<s>\<e> P \<Longrightarrow> \<^bold>a\<^bold>r\<^bold>g\<^bold>u\<^bold>m\<^bold>e\<^bold>n\<^bold>t A \<s>\<h>\<i>\<f>\<t>\<s> Ya \<w>\<i>\<t>\<h> PA)
 \<Longrightarrow> (\<p>\<r>\<e>\<m>\<i>\<s>\<e> \<not> P \<Longrightarrow> \<^bold>a\<^bold>r\<^bold>g\<^bold>u\<^bold>m\<^bold>e\<^bold>n\<^bold>t B \<s>\<h>\<i>\<f>\<t>\<s> Yb \<w>\<i>\<t>\<h> PB)
 \<Longrightarrow> If P Ya Yb \<t>\<r>\<a>\<n>\<s>\<f>\<o>\<r>\<m>\<s> Y @action invoke_branch_convergence
-\<Longrightarrow> If P A B \<s>\<h>\<i>\<f>\<t>\<s> Y \<w>\<i>\<t>\<h> If P PA PB @action \<A>_action_case\<close>
+\<Longrightarrow> If P A B \<s>\<h>\<i>\<f>\<t>\<s> Y \<w>\<i>\<t>\<h> If P PA PB @action \<A>case (If P A B)\<close>
   unfolding Argument_def Action_Tag_def Premise_def
   apply (cases P; simp)
   using \<phi>view_trans view_shift_by_implication apply fastforce
   using View_Shift_def view_shift_by_implication by force
 
-lemma [\<phi>reason 1000]:
+lemma [\<phi>reason 1000 for \<open>If _ _ _ \<t>\<r>\<a>\<n>\<s>\<f>\<o>\<r>\<m>\<s> _ \<w>\<i>\<t>\<h> _ @action \<A>case (If _ _ _)\<close>
+                        \<open>If _ _ _ \<t>\<r>\<a>\<n>\<s>\<f>\<o>\<r>\<m>\<s> _ \<w>\<i>\<t>\<h> _ @action \<A>case ?var\<close>]:
   \<open> (\<p>\<r>\<e>\<m>\<i>\<s>\<e> P \<Longrightarrow> \<^bold>a\<^bold>r\<^bold>g\<^bold>u\<^bold>m\<^bold>e\<^bold>n\<^bold>t A \<t>\<r>\<a>\<n>\<s>\<f>\<o>\<r>\<m>\<s> Ya \<w>\<i>\<t>\<h> PA)
 \<Longrightarrow> (\<p>\<r>\<e>\<m>\<i>\<s>\<e> \<not> P \<Longrightarrow> \<^bold>a\<^bold>r\<^bold>g\<^bold>u\<^bold>m\<^bold>e\<^bold>n\<^bold>t B \<t>\<r>\<a>\<n>\<s>\<f>\<o>\<r>\<m>\<s> Yb \<w>\<i>\<t>\<h> PB)
 \<Longrightarrow> \<^bold>d\<^bold>o If P Ya Yb \<t>\<r>\<a>\<n>\<s>\<f>\<o>\<r>\<m>\<s> Y @action invoke_branch_convergence
-\<Longrightarrow> If P A B \<t>\<r>\<a>\<n>\<s>\<f>\<o>\<r>\<m>\<s> Y \<w>\<i>\<t>\<h> If P PA PB @action \<A>_action_case\<close>
+\<Longrightarrow> If P A B \<t>\<r>\<a>\<n>\<s>\<f>\<o>\<r>\<m>\<s> Y \<w>\<i>\<t>\<h> If P PA PB @action \<A>case (If P A B)\<close>
   unfolding Argument_def Action_Tag_def Premise_def
   apply (cases P; simp)
   using implies_trans apply fastforce
   using implies_trans by fastforce
+
+lemma [\<phi>reason default 0]:
+  \<open> FAIL TEXT(\<open>Don't know how to case split\<close> X)
+\<Longrightarrow> X \<t>\<r>\<a>\<n>\<s>\<f>\<o>\<r>\<m>\<s> Y \<w>\<i>\<t>\<h> Any @action \<A>case Any'\<close>
+  by blast
 
 
 (*lemma [\<phi>reason 1000]:
@@ -776,13 +789,13 @@ consts action_dup    :: \<open>action\<close>
        action_drop   :: \<open>action\<close>
 
 lemma dup_\<phi>app:
-  \<open>PROP Call_Action (\<A>_transformation (\<A>_leading_item (\<A>_structural_1_2 action_dup)))\<close> ..
+  \<open>Call_Action (\<A>_transformation (\<A>_leading_item (\<A>_structural_1_2 action_dup)))\<close> ..
 
 lemma shrink_\<phi>app:
-  \<open>PROP Call_Action (\<A>_transformation (multi_arity (\<A>_structural_2_1 action_shrink)))\<close> ..
+  \<open>Call_Action (\<A>_transformation (multi_arity (\<A>_structural_2_1 action_shrink)))\<close> ..
 
 lemma drop_\<phi>app:
-  \<open>PROP Call_Action (\<A>_view_shift_or_imp (multi_arity action_drop))\<close> ..
+  \<open>Call_Action (\<A>_view_shift_or_imp (multi_arity action_drop))\<close> ..
 
 (*subsection \<open>Simplification as an Action\<close>
 
